Refactoring to use Definitions

Access.v
@@ -1,5 +1,163 @@
-From Elo Require Export AccessCore.
-From Elo Require Export NotAccess.
-From Elo Require Export AccessExtra.
-From Elo Require Export UnsafeAccess.
+From Elo Require Import Util.
+From Elo Require Import Array.
+From Elo Require Import Core.
+
+(* ------------------------------------------------------------------------- *)
+(* access                                                                    *)
+(* ------------------------------------------------------------------------- *)
+
+(*
+  A term has access to an address if it refers to the address directly or 
+  indirectly.
+  
+  Ignores <spawn> blocks.
+*)
+Inductive access (ad : addr) (m : mem) : tm -> Prop :=
+  | acc_mem : forall ad' T,
+    ad <> ad' ->
+    access ad m m[ad'].tm ->
+    access ad m <{&ad' :: T}>
+
+  | acc_ad : forall T,
+    access ad m <{&ad :: T}>
+
+  | acc_new : forall T t,
+    access ad m t ->
+    access ad m <{new T t}>
+
+  | acc_load : forall t,
+    access ad m t ->
+    access ad m <{*t}>
+
+  | acc_asg1 : forall t1 t2,
+    access ad m t1 ->
+    access ad m <{t1 = t2}>
+
+  | acc_asg2 : forall t1 t2,
+    access ad m t2 ->
+    access ad m <{t1 = t2}>
+
+  | acc_fun : forall x Tx t,
+    access ad m t ->
+    access ad m <{fn x Tx t}>
+
+  | acc_call1 : forall t1 t2,
+    access ad m t1 ->
+    access ad m <{call t1 t2}>
+
+  | acc_call2 : forall t1 t2,
+    access ad m t2 ->
+    access ad m <{call t1 t2}>
+
+  | acc_seq1 : forall t1 t2,
+    access ad m t1 ->
+    access ad m <{t1; t2}>
+
+  | acc_seq2 : forall t1 t2,
+    access ad m t2 ->
+    access ad m <{t1; t2}>
+  .
+
+(* ------------------------------------------------------------------------- *)
+(* valid-accesses                                                            *)
+(* ------------------------------------------------------------------------- *)
+
+(*
+  A term has valid accesses if all the addresses it has access to are within
+  the bounds of the memory.
+*)
+Definition valid_accesses (m : mem) (t : tm) :=
+  forall ad, access ad m t -> ad < #m.
+
+(* ------------------------------------------------------------------------- *)
+(* unfold hints                                                              *)
+(* ------------------------------------------------------------------------- *)
+
+#[export] Hint Unfold valid_accesses : vac.
+
+#[export] Hint Extern 4 => unfold valid_accesses : vac.
+
+(* ------------------------------------------------------------------------- *)
+(* access inversion                                                          *)
+(* ------------------------------------------------------------------------- *)
+
+Local Ltac match_acc tactic :=
+  match goal with
+  | H : access _ _ thread_default |- _ => tactic H
+  | H : access _ _ <{unit    }>   |- _ => tactic H
+  | H : access _ _ <{N _     }>   |- _ => tactic H
+  | H : access _ _ <{& _ :: _}>   |- _ => tactic H
+  | H : access _ _ <{new _ _ }>   |- _ => tactic H
+  | H : access _ _ <{* _     }>   |- _ => tactic H
+  | H : access _ _ <{_ = _   }>   |- _ => tactic H
+  | H : access _ _ <{var _   }>   |- _ => tactic H
+  | H : access _ _ <{fn _ _ _}>   |- _ => tactic H
+  | H : access _ _ <{call _ _}>   |- _ => tactic H
+  | H : access _ _ <{_ ; _   }>   |- _ => tactic H
+  | H : access _ _ <{spawn _ }>   |- _ => tactic H
+  end.
+
+Ltac inv_acc := match_acc inv.
+
+Ltac inv_clear_acc := match_acc inv_clear.
+
+(* ------------------------------------------------------------------------- *)
+(* valid-accesses inversion                                                  *)
+(* ------------------------------------------------------------------------- *)
+
+Local Ltac solve_vac_inversion := 
+  intros; autounfold with vac in *; try split; eauto using access.
+
+Local Lemma inv_vac_ad : forall m ad T,
+  valid_accesses m <{&ad :: T}> ->
+  ad < #m /\ valid_accesses m m[ad].tm.
+Proof.
+  solve_vac_inversion. intros ad'.
+  destruct (nat_eq_dec ad ad'); subst; eauto using access.
+Qed.
+
+Local Lemma inv_vac_new : forall m t T,
+  valid_accesses m <{new T t}> ->
+  valid_accesses m t.
+Proof. solve_vac_inversion. Qed.
+
+Local Lemma inv_vac_load : forall m t,
+  valid_accesses m <{*t}> ->
+  valid_accesses m t.
+Proof. solve_vac_inversion. Qed.
+
+Local Lemma inv_vac_asg : forall m t1 t2,
+  valid_accesses m <{t1 = t2}> ->
+  valid_accesses m t1 /\ valid_accesses m t2.
+Proof. solve_vac_inversion. Qed.
+
+Local Lemma inv_vac_fun : forall m x Tx t,
+  valid_accesses m <{fn x Tx t}> ->
+  valid_accesses m t.
+Proof. solve_vac_inversion. Qed.
+
+Local Lemma inv_vac_call : forall m t1 t2,
+  valid_accesses m <{call t1 t2}> ->
+  valid_accesses m t1 /\ valid_accesses m t2.
+Proof. solve_vac_inversion. Qed.
+
+Local Lemma inv_vac_seq : forall m t1 t2,
+  valid_accesses m <{t1; t2}> ->
+  valid_accesses m t1 /\ valid_accesses m t2.
+Proof. solve_vac_inversion. Qed.
+
+Ltac inv_vac :=
+  match goal with
+  (* irrelevant for unit  *)
+  (* irrelevant for num   *)
+  | H : valid_accesses _ <{& _ :: _}> |- _ => eapply inv_vac_ad   in H as [? ?]
+  | H : valid_accesses _ <{new _ _ }> |- _ => eapply inv_vac_new  in H
+  | H : valid_accesses _ <{* _     }> |- _ => eapply inv_vac_load in H
+  | H : valid_accesses _ <{_ = _   }> |- _ => eapply inv_vac_asg  in H as [? ?]
+  (* irrelevant for var   *)                    
+  | H : valid_accesses _ <{fn _ _ _}> |- _ => eapply inv_vac_fun  in H
+  | H : valid_accesses _ <{call _ _}> |- _ => eapply inv_vac_call in H as [? ?]
+  | H : valid_accesses _ <{_ ; _   }> |- _ => eapply inv_vac_seq  in H as [? ?]
+  (* irrelevant for spawn *)                    
+  end.
 
