ConsistentlyTypedReferences.v
@@ -1,0 +1,84 @@
+From Elo Require Import Util.
+From Elo Require Import Array.
+From Elo Require Import Map.
+From Elo Require Import Core.
+
+(* ------------------------------------------------------------------------- *)
+(* consistently-typed-references                                             *)
+(* ------------------------------------------------------------------------- *)
+
+Inductive consistently_typed_references (m : mem) : tm -> Prop :=
+  | ctr_unit :
+    consistently_typed_references m <{unit}> 
+
+  | ctr_num : forall n,
+    consistently_typed_references m <{N n}>
+
+  | ctr_refM : forall T ad,
+    empty |-- m[ad].tm is T ->
+    m[ad].typ = <{{ &T }}> ->
+    consistently_typed_references m <{&ad :: &T}>
+
+  | ctr_refI : forall T ad,
+    empty |-- m[ad].tm is <{{ Immut T }}> ->
+    m[ad].typ = <{{ i&T }}> ->
+    consistently_typed_references m <{&ad :: i&T}>
+
+  | ctr_new : forall T t,
+    consistently_typed_references m t ->
+    consistently_typed_references m <{new T t}> 
+
+  | ctr_load : forall t,
+    consistently_typed_references m t ->
+    consistently_typed_references m <{*t}> 
+
+  | ctr_asg : forall t1 t2,
+    consistently_typed_references m t1 ->
+    consistently_typed_references m t2 ->
+    consistently_typed_references m <{t1 = t2}> 
+
+  | ctr_var : forall x,
+    consistently_typed_references m <{var x}>
+
+  | ctr_fun : forall x Tx t,
+    consistently_typed_references m t ->
+    consistently_typed_references m <{fn x Tx t}>
+
+  | ctr_call : forall t1 t2,
+    consistently_typed_references m t1 ->
+    consistently_typed_references m t2 ->
+    consistently_typed_references m <{call t1 t2}> 
+
+  | ctr_seq : forall t1 t2,
+    consistently_typed_references m t1 ->
+    consistently_typed_references m t2 ->
+    consistently_typed_references m <{t1; t2}>
+
+  | ctr_spawn : forall t,
+    consistently_typed_references m t ->
+    consistently_typed_references m <{spawn t}>
+  .
+
+(* ------------------------------------------------------------------------- *)
+(* inversion                                                                 *)
+(* ------------------------------------------------------------------------- *)
+
+Local Ltac match_ctr tactic :=
+  match goal with
+  (* irrelevant for unit *)
+  (* irrelevant for num  *)
+  | H : consistently_typed_references _ <{& _ :: _}> |- _ => tactic H
+  | H : consistently_typed_references _ <{new _ _ }> |- _ => tactic H
+  | H : consistently_typed_references _ <{* _     }> |- _ => tactic H
+  | H : consistently_typed_references _ <{_ = _   }> |- _ => tactic H
+  (* irrelevant for var  *)
+  | H : consistently_typed_references _ <{fn _ _ _}> |- _ => tactic H
+  | H : consistently_typed_references _ <{call _ _}> |- _ => tactic H
+  | H : consistently_typed_references _ <{_ ; _   }> |- _ => tactic H
+  | H : consistently_typed_references _ <{spawn _ }> |- _ => tactic H
+  end.
+
+Ltac inv_ctr := match_ctr inv.
+
+Ltac inv_clear_ctr := match_ctr inv_clear.
+
