Definitions.v
@@ -1,0 +1,6 @@
+From Elo Require Export ValidAddresses.
+From Elo Require Export WellTypedTerm.
+From Elo Require Export ConsistentlyTypedReferences.
+From Elo Require Export Access.
+From Elo Require Export NotAccess.
+From Elo Require Export UnsafeAccess.
