NotAccess.v
@@ -1,12 +1,6 @@
-From Coq Require Import Arith.Arith.
-From Coq Require Import Lia.
-
 From Elo Require Import Util.
-From Elo Require Import Array.
 From Elo Require Import Core.
-From Elo Require Import CoreExt.
-From Elo Require Import ValidAddresses.
-From Elo Require Import AccessCore.
+From Elo Require Import Access.
 
 Inductive not_access (ad : addr) (m : mem) : tm -> Prop :=
   | nacc_unit :
@@ -54,6 +48,10 @@ Inductive not_access (ad : addr) (m : mem) : tm -> Prop :=
     not_access ad m <{spawn t}>
   .
 
+(* ------------------------------------------------------------------------- *)
+(* inversion                                                                 *)
+(* ------------------------------------------------------------------------- *)
+
 Theorem nacc_iff : forall m t ad,
   ~ access ad m t <-> not_access ad m t.
 Proof.
@@ -71,185 +69,28 @@ Proof.
   eauto using access.
 Qed.
 
-(* ------------------------------------------------------------------------- *)
-(* inversion                                                                 *)
-(* ------------------------------------------------------------------------- *)
+Local Ltac manual_inv_nacc Hnacc :=
+  eapply nacc_iff in Hnacc; inv Hnacc; eauto using access.
 
-Ltac inv_nacc Hnacc :=
-  eapply nacc_iff in Hnacc; inversion Hnacc; subst; eauto using access.
+Local Ltac manual_inv_clear_nacc Hnacc :=
+  manual_inv_nacc; clear Hnacc.
 
-(* ------------------------------------------------------------------------- *)
-(* length                                                                    *)
-(* ------------------------------------------------------------------------- *)
+Local Ltac match_nacc tactic :=
+  match goal with
+  (* irrelevant for unit  *)
+  (* irrelevant for num   *)
+  | H : ~ access _ _ <{& _ :: _}>   |- _ => tactic H
+  | H : ~ access _ _ <{new _ _ }>   |- _ => tactic H
+  | H : ~ access _ _ <{* _     }>   |- _ => tactic H
+  | H : ~ access _ _ <{_ = _   }>   |- _ => tactic H
+  (* irrelevant for var   *)
+  | H : ~ access _ _ <{fn _ _ _}>   |- _ => tactic H
+  | H : ~ access _ _ <{call _ _}>   |- _ => tactic H
+  | H : ~ access _ _ <{_ ; _   }>   |- _ => tactic H
+  (* irrelevant for spawn *)
+  end.
 
-Lemma nacc_vad_length : forall m t,
-  forall_memory m (valid_addresses m) ->
-  valid_addresses m t ->
-  ~ access (#m) m t.
-Proof.
-  intros * ? Hvad Hacc. remember (#m) as ad.
-  induction Hacc; inversion_vad; eauto. lia.
-Qed.
+Ltac inv_nacc := match_nacc manual_inv_nacc.
 
-(* ------------------------------------------------------------------------- *)
-(* preservation                                                              *)
-(* ------------------------------------------------------------------------- *)
-
-Local Lemma nacc_subst_preservation : forall m t tx ad x,
-  ~ access ad m t ->
-  ~ access ad m tx ->
-  ~ access ad m ([x := tx] t).
-Proof.
-  intros * Hnacc ?. induction t; simpl;
-  try solve [inv_nacc Hnacc; eapply nacc_iff; eauto using not_access];
-  destruct string_eq_dec; trivial.
-  inv_nacc Hnacc. eapply nacc_iff. eauto using not_access.
-Qed.
-
-Lemma nacc_mem_add_preservation : forall m t ad vT,
-  ~ access (#m) m t ->
-  ~ access ad m t ->
-  ~ access ad (m +++ vT) t.
-Proof.
-  intros * Hnacc1 Hnacc2 Hacc. induction Hacc; inv_nacc Hnacc2.
-  decompose sum (lt_eq_lt_dec ad' (#m)); subst; simpl_array;
-  inv_nacc Hnacc1. eapply IHHacc; eapply nacc_iff; eauto using not_access.
-Qed.
-
-Local Lemma nacc_mem_set_preservation : forall m t ad ad' v T,
-  ~ access ad m v ->
-  ~ access ad m t ->
-  ~ access ad m[ad' <- (v, T)] t.
-Proof.
-  assert (forall m ad ad' v,
-    access ad m[ad' <- v] m[ad' <- v][ad'].tm -> ad' < length m). {
-      intros * H. eapply not_ge. rewrite ge_iff_le. intros ?.
-      rewrite (get_set_invalid memory_default) in H; trivial. inversion H.
-  }
-  (* main proof *)
-  intros * ? ? Hacc. induction Hacc; eauto using access.
-  match goal with _ : _ <> ?ad |- _ => rename ad into ad'' end. 
-  destruct (nat_eq_dec ad' ad''); subst;
-  try (assert (ad'' < #m) by eauto);
-  simpl_array; eauto using access.
-Qed.
-
-(* alternative for mem_set ------------------------------------------------- *)
-
-Lemma alt_nacc_mem_set_preservation : forall m t ad ad' vT,
-  ~ access ad' m t ->
-  ~ access ad m t ->
-  ~ access ad m[ad' <- vT] t.
-Proof.
-  intros * Hnacc' Hnacc Hacc.
-  induction Hacc; inv_nacc Hnacc'; inv_nacc Hnacc.
-  simpl_array. eauto.
-Qed.
-
-(* tstep ------------------------------------------------------------------- *)
-
-Local Lemma nacc_tstep_none_preservation : forall m t t' ad,
-  ~ access ad m t ->
-  t --[EF_None]--> t' ->
-  ~ access ad m t'.
-Proof.
-  intros * Hnacc. intros. induction_step; inv_nacc Hnacc;
-  try solve [eapply nacc_iff; eauto using not_access].
-  match goal with H : ~ access _ _ <{ fn _ _ _ }> |- _ => inv_nacc H end.
-  eauto using nacc_subst_preservation.
-Qed.
-
-Local Lemma nacc_tstep_alloc_preservation : forall m t t' ad v T,
-  ad < #m ->
-  forall_memory m (valid_addresses m) ->
-  valid_addresses m t ->
-  ~ access ad m t ->
-  t --[EF_Alloc (#m) v T]--> t' ->
-  ~ access ad (m +++ (v, T)) t'.
-Proof.
-  intros * ? ? ? Hnacc ?.
-  induction_step; inversion_vad; inv_nacc Hnacc; eapply nacc_iff;
-  eauto using not_access, nacc_mem_add_preservation, nacc_vad_length.
-  eapply nacc_ad. eauto using not_eq_sym, Nat.lt_neq.
-  simpl_array. eauto using nacc_mem_add_preservation, nacc_vad_length.
-Qed.
-
-Local Lemma nacc_tstep_read_preservation : forall m t t' ad ad',
-  ~ access ad m t ->
-  t --[EF_Read ad' m[ad'].tm]--> t' ->
-  ~ access ad m t'.
-Proof.
-  intros * Hnacc ?. induction_step; inv_nacc Hnacc;
-  try solve [eapply nacc_iff; eauto using not_access].
-  match goal with H : ~ access _ _ _ |- _ => inv_nacc H end.
-Qed.
-
-Local Lemma nacc_tstep_write_preservation : forall m t t' ad ad' v T,
-  ~ access ad m t ->
-  t --[EF_Write ad' v T]--> t' ->
-  ~ access ad m[ad' <- (v, T)] t'.
-Proof.
-  assert (forall m t t' ad ad' v T,
-    ~ access ad m t ->
-    t --[EF_Write ad' v T]--> t' ->
-    ~ access ad m v)
-    by (intros; induction_step; eauto using access).
-  (* main proof *)
-  intros * Hnacc ?. induction_step; inv_nacc Hnacc;
-  eapply nacc_iff; eauto using not_access, nacc_mem_set_preservation.
-Qed.
-
-Lemma nacc_tstep_spawn_preservation : forall m t t' block ad,
-  ~ access ad m t ->
-  t --[EF_Spawn block]--> t' ->
-  ~ access ad m t'.
-Proof.
-  intros * Hnacc ?. induction_step; inv_nacc Hnacc;
-  eapply nacc_iff; eauto using not_access.
-Qed.
-
-Corollary nacc_mstep_preservation : forall m m' t t' e ad,
-  forall_memory m (valid_addresses m) ->
-  valid_addresses m t ->
-  (* --- *)
-  ad < #m ->
-  ~ access ad m t ->
-  m / t ==[e]==> m' / t' ->
-  ~ access ad m' t'.
-Proof.
-  intros. inversion_mstep;
-  eauto using nacc_tstep_none_preservation,
-    nacc_tstep_alloc_preservation,
-    nacc_tstep_read_preservation,
-    nacc_tstep_write_preservation.
-Qed.
-
-(* cstep ------------------------------------------------------------------- *)
-
-Local Lemma nacc_thread_default_preservation : forall m ad,
-  ~ access ad m thread_default.
-Proof.
-  intros. eapply nacc_iff. eauto using not_access.
-Qed.
-
-Local Lemma nacc_spawn_block_preservation : forall m t t' block ad,
-  ~ access ad m t ->
-  t --[EF_Spawn block]--> t' ->
-  access ad m block ->
-  exists T, m[ad].typ = <{{ i&T }}>.
-Proof.
-  (* need SafeSpawns to prove this. *)
-Abort.
-
-Local Lemma nacc_untouched_threads_preservation :
-  forall m m' ths tid tid' t' e ad,
-    forall_memory m (valid_addresses m) ->
-    forall_threads ths (valid_addresses m) ->
-    tid <> tid' ->
-    ~ access ad m ths[tid'] ->
-    m / ths[tid] ==[e]==> m' / t' ->
-    ~ access ad m' ths[tid'].
-Proof.
-  (* nees SMS to prove this. *)
-Abort.
+Ltac inv_clear_nacc := match_nacc manual_inv_clear_nacc.
 
