SsPreservation.v
@@ -1,0 +1,156 @@
+
+(* ------------------------------------------------------------------------- *)
+(* SafeSpawns mstep term preservation                                        *)
+(* ------------------------------------------------------------------------- *)
+
+Local Lemma safe_spawns_subst : forall Gamma x t v T Tx,
+  value v ->
+  empty |-- v is Tx ->
+  Gamma[x <== Tx] |-- t is T ->
+  SafeSpawns v ->
+  SafeSpawns t ->
+  SafeSpawns ([x := v] t).
+Proof.
+  assert (H1 : forall Gamma x T,
+    (safe Gamma[x <== <{{ &T }}>]) x = None);
+  assert (H2 : forall Gamma x T T',
+    (safe Gamma[x <== <{{ T --> T' }}>]) x = None);
+  try solve [unfold safe; intros; rewrite lookup_update_eq; reflexivity].
+  (* main proof *)
+  intros * Hvalue HtypeV HtypeT Hssv Hsst.
+  generalize dependent Gamma. generalize dependent T. generalize dependent Tx.
+  induction Hsst; intros; inversion_type;
+  simpl; try (destruct string_eq_dec);
+  eauto using SafeSpawns, equivalence_typing, MapEquivalence.update_permutation.
+  eapply safe_spawns_spawn. destruct (hasvar_dec x t).
+  - eapply nomut_subst; trivial.
+    inversion Hvalue; subst; eauto using NoMut.
+    + inversion HtypeV; subst; eauto using NoMut.
+      exfalso. eapply hasvar_typing; eauto using H1.
+    + inversion_clear Hvalue. inversion HtypeV; subst.
+      exfalso. eapply hasvar_typing; eauto using H2. 
+  - erewrite hasvar_subst; eauto.
+Qed.
+
+Local Lemma mstep_tm_safe_spawns_preservation : forall m m' t t' eff T,
+  empty |-- t is T ->
+  forall_memory m SafeSpawns ->
+  SafeSpawns t ->
+  m / t ==[eff]==> m' / t' ->
+  SafeSpawns t'.
+Proof.
+  intros. generalize dependent T.
+  inversion_clear_mstep; induction_step; intros;
+  try solve [inversion_type; inversion_ss; eauto using SafeSpawns].
+  do 2 (inversion_ss; inversion_type).
+  eauto using safe_spawns_subst.
+Qed.
+
+(* ------------------------------------------------------------------------- *)
+(* SafeSpawns mstep memory preservation                                      *)
+(* ------------------------------------------------------------------------- *)
+
+Local Lemma mem_safe_spawns_alloc : forall m t t' v V,
+  forall_memory m SafeSpawns ->
+  SafeSpawns t ->
+  t --[EF_Alloc (length m) v V]--> t' ->
+  forall_memory (m +++ (v, V)) SafeSpawns.
+Proof.
+  intros. assert (SafeSpawns v) by (induction_step; inversion_ss; eauto).
+  unfold forall_memory. eauto using forall_array_add, SafeSpawns.
+Qed.
+
+Local Lemma mem_safe_spawns_store : forall m t t' ad v V,
+  forall_memory m SafeSpawns ->
+  SafeSpawns t ->
+  t --[EF_Write ad v V]--> t' ->
+  forall_memory m[ad <- (v, V)] SafeSpawns.
+Proof.
+  intros. assert (SafeSpawns v) by (induction_step; inversion_ss; eauto).
+  unfold forall_memory. eauto using forall_array_set, SafeSpawns.
+Qed.
+
+Local Lemma mstep_mem_safe_spawns_preservation : forall m m' t t' eff,
+  forall_memory m SafeSpawns ->
+  SafeSpawns t ->
+  m / t ==[eff]==> m' / t' ->
+  forall_memory m' SafeSpawns.
+Proof.
+  intros. inversion_mstep;
+  eauto using mem_safe_spawns_alloc, mem_safe_spawns_store.
+Qed.
+
+(* ------------------------------------------------------------------------- *)
+(* SafeSpawns cstep preservation                                             *)
+(* ------------------------------------------------------------------------- *)
+
+Local Lemma nomut_then_safe_spawns : forall t,
+  NoMut t ->
+  SafeSpawns t.
+Proof.
+  intros * H. induction t; induction H; eauto using SafeSpawns.
+Qed.
+
+Local Lemma safe_spawns_for_block : forall t t' block,
+  SafeSpawns t ->
+  t --[EF_Spawn block]--> t' ->
+  SafeSpawns block.
+Proof.
+  intros. induction_step; inversion_ss;
+  eauto using SafeSpawns, nomut_then_safe_spawns.
+Qed.
+
+Local Lemma step_safe_spawns_preservation : forall t t' block,
+  SafeSpawns t ->
+  t --[EF_Spawn block]--> t' ->
+  SafeSpawns t'.
+Proof.
+  intros. induction_step; inversion_ss;
+  eauto using SafeSpawns, nomut_then_safe_spawns.
+Qed.
+
+Theorem safe_spawns_preservation : forall m m' ths ths' tid eff,
+  forall_program m ths well_typed_term ->
+  (* --- *)
+  forall_program m ths SafeSpawns ->
+  m / ths ~~[tid, eff]~~> m' / ths' ->
+  forall_program m' ths' SafeSpawns.
+Proof.
+  intros * [_ Htype] [? ?]. split; inversion_cstep;
+  eauto using mstep_mem_safe_spawns_preservation.
+  - eapply forall_array_add; eauto using SafeSpawns, safe_spawns_for_block.
+    eapply forall_array_set;
+    eauto using SafeSpawns, step_safe_spawns_preservation.
+  - eapply forall_array_set;
+    eauto using SafeSpawns. specialize (Htype tid) as [? ?].
+    eauto using mstep_tm_safe_spawns_preservation. (* performance *)
+Qed.
+
+(* ------------------------------------------------------------------------- *)
+(*                                                                           *)
+(* ------------------------------------------------------------------------- *)
+
+Local Lemma nomut_block : forall t t' block,
+  SafeSpawns t ->
+  t --[EF_Spawn block]--> t' ->
+  NoMut block.
+Proof.
+  intros. induction_step; inversion_ss; eauto.
+Qed.
+
+Local Lemma nomut_then_nuacc: forall m t ad,
+  NoMut t ->
+  unsafe_access ad m t ->
+  False.
+Proof.
+  intros * Hnm Huacc. induction Hnm; inv_uacc; eauto.
+Qed.
+
+Theorem nuacc_spawn_block : forall m t t' block ad,
+  SafeSpawns t ->
+  t --[EF_Spawn block]--> t' ->
+  ~ unsafe_access ad m block.
+Proof.
+  eauto using nomut_block, nomut_then_nuacc.
+Qed.
+
