UnsafeAccess.v
@@ -1,15 +1,5 @@
-From Coq Require Import Arith.Arith.
-From Coq Require Import Lia.
-
 From Elo Require Import Util.
-From Elo Require Import Array.
-From Elo Require Import Map.
 From Elo Require Import Core.
-From Elo Require Import CoreExt.
-From Elo Require Import ValidAddresses.
-From Elo Require Import References.
-From Elo Require Import AccessCore.
-From Elo Require Import NotAccess.
 
 (* ------------------------------------------------------------------------- *)
 (* unsafe-access                                                             *)
@@ -87,61 +77,26 @@ Ltac inv_uacc := match_uacc inv.
 Ltac inv_clear_uacc := match_uacc inv_clear.
 
 (* ------------------------------------------------------------------------- *)
-(* unsafe-access dec                                                         *)
-(* ------------------------------------------------------------------------- *)
-
-Lemma uacc_dec : forall m t ad,
-  Decidable.decidable (unsafe_access ad m t).
-Proof. eauto using classic_decidable. Qed.
-
-(* ------------------------------------------------------------------------- *)
-(* unsafe-access inheritance                                                 *)
-(* ------------------------------------------------------------------------- *)
-
-Lemma uacc_mem_add_inheritance : forall m t ad vT,
-  ~ access (#m) m t ->
-  unsafe_access ad (m +++ vT) t ->
-  unsafe_access ad m t.
-Proof.
-  intros * Hnacc Huacc. induction Huacc; subst; inv_nacc Hnacc;
-  eauto using unsafe_access.
-  eapply uacc_mem; trivial.
-  decompose sum (lt_eq_lt_dec ad' (#m)); subst; simpl_array; eauto; lia.
-Qed.
-
-Lemma uacc_mem_set_inheritance : forall m t ad ad' vT,
-  ~ access ad' m t ->
-  unsafe_access ad m[ad' <- vT] t ->
-  unsafe_access ad m t.
-Proof.
-  intros * Hnacc Huacc. induction Huacc; inv_nacc Hnacc;
-  eauto using unsafe_access. simpl_array. eauto using unsafe_access.
-Qed.
-
-Local Lemma uacc_tstep_spawn_inheritance : forall m t t' block ad,
-  unsafe_access ad m t' ->
-  t --[EF_Spawn block]--> t' ->
-  unsafe_access ad m t.
-Proof.
-  intros. induction_step; inv_uacc; eauto using unsafe_access.
-Qed.
-
-(* ------------------------------------------------------------------------- *)
 (* not-unsafe-access inversion                                               *)
 (* ------------------------------------------------------------------------- *)
 
-Lemma nuacc_unit : forall m ad,
-  ~ unsafe_access ad m <{unit}>.
-Proof. intros * ?. inv_uacc. Qed.
+Local Lemma inv_nuacc_ad_eq : forall m ad T,
+  ~ unsafe_access ad m <{&ad :: &T}> ->
+  False.
+Proof.
+  intros. eauto using unsafe_access.
+Qed.
+
+Local Lemma inv_nuacc_ad_neq : forall m ad ad' T,
+  ~ unsafe_access ad m <{&ad' :: &T}> ->
+  (ad <> ad' /\ ~ unsafe_access ad m m[ad'].tm).
+Proof.
+  intros. destruct (nat_eq_dec ad ad'); subst; eauto using unsafe_access.
+  exfalso. eauto using inv_nuacc_ad_eq.
+Qed.
 
 Local Ltac solve_nuacc_inversion :=
   intros; try (split; intros); eauto using unsafe_access.
-
-Local Lemma inv_nuacc_mem : forall m ad ad' T,
-  ad <> ad' ->
-  ~ unsafe_access ad m <{&ad' :: &T}> ->
-  ~ unsafe_access ad m (m[ad'].tm).
-Proof. solve_nuacc_inversion. Qed.
 
 Local Lemma inv_nuacc_new : forall m t ad T,
   ~ unsafe_access ad m <{new T t}> ->
@@ -175,256 +130,21 @@ Proof. solve_nuacc_inversion. Qed.
 
 Ltac inv_nuacc :=
   match goal with
-  | H : ~ unsafe_access ?ad _ <{ & ?ad' ::   _ }>, Hneq : ?ad <> ?ad' |- _ =>
-    eapply (inv_nuacc_mem _ _ _ _ Hneq) in H
-  | H : ~ unsafe_access ?ad _ <{ & ?ad  :: & _ }> |- _ =>
-    contradict H; eauto using unsafe_access
-  | H : ~ unsafe_access _ _   <{ new _ _       }> |- _ =>
-    eapply inv_nuacc_new  in H
-  | H : ~ unsafe_access _ _   <{ * _           }> |- _ =>
-    eapply inv_nuacc_load in H
-  | H : ~ unsafe_access _ _   <{ _ = _         }> |- _ =>
-    eapply inv_nuacc_asg  in H as [? ?]
-  | H : ~ unsafe_access _ _   <{ fn _ _ _      }> |- _ =>
-    eapply inv_nuacc_fun  in H
-  | H : ~ unsafe_access _ _   <{ call _ _      }> |- _ =>
-    eapply inv_nuacc_call in H as [? ?]
-  | H : ~ unsafe_access _ _   <{ _ ; _         }> |- _ =>
-    eapply inv_nuacc_seq  in H as [? ?]
+  | H : ~ unsafe_access ?ad _ <{& ?ad  :: & _}> |- _ =>
+    eapply inv_nuacc_ad_eq  in H; solve contradiction
+  | H : ~ unsafe_access ?ad _ <{& ?ad' ::   _}> |- _ =>
+    eapply inv_nuacc_ad_neq in H as [? ?]
+  | H : ~ unsafe_access _ _   <{new _ _      }> |- _ =>
+    eapply inv_nuacc_new    in H
+  | H : ~ unsafe_access _ _   <{* _          }> |- _ =>
+    eapply inv_nuacc_load   in H
+  | H : ~ unsafe_access _ _   <{_ = _        }> |- _ =>
+    eapply inv_nuacc_asg    in H as [? ?]
+  | H : ~ unsafe_access _ _   <{fn _ _ _     }> |- _ =>
+    eapply inv_nuacc_fun    in H
+  | H : ~ unsafe_access _ _   <{call _ _     }> |- _ =>
+    eapply inv_nuacc_call   in H as [? ?]
+  | H : ~ unsafe_access _ _   <{_ ; _        }> |- _ =>
+    eapply inv_nuacc_seq    in H as [? ?]
   end.
-
-(* ------------------------------------------------------------------------- *)
-(* important properties and lemmas                                           *)
-(* ------------------------------------------------------------------------- *)
-
-(* unsafe-access ----------------------------------------------------------- *)
-
-Local Theorem uacc_soundness : forall m m' t t' ad e T,
-  ad < #m ->
-  empty |-- t is T ->
-  ~ unsafe_access ad m t ->
-  m / t ==[e]==> m' / t' ->
-  m[ad].tm = m'[ad].tm.
-Proof.
-  intros. rename ad into ad'. inversion_clear_mstep; trivial.
-  - decompose sum (lt_eq_lt_dec ad' (#m)); subst; simpl_array; trivial. lia.
-  - decompose sum (lt_eq_lt_dec ad' ad); subst; simpl_array; trivial.
-    generalize dependent T.
-    induction_step; intros; inversion_type; inv_nuacc; eauto.
-    inversion_type. exfalso. eauto using unsafe_access.
-Qed.
-
-Lemma uacc_then_acc : forall m t ad,
-  unsafe_access ad m t ->
-  access ad m t.
-Proof.
-  intros * Huacc. induction Huacc; eauto using access.
-Qed.
-
-Theorem immutable_reference_then_nuacc : forall m ad v T,
-  value v ->
-  empty |-- v is <{{Immut T}}> ->
-  unsafe_access ad m v ->
-  False.
-Proof.
-  intros * Hval ? ?. destruct Hval;
-  inversion_type; inv_uacc; eauto using unsafe_access.
-Qed.
-
-Local Lemma nuacc_from_nacc : forall m t ad,
-  ~ access ad m t ->
-  ~ unsafe_access ad m t.
-Proof.
-  intros * ? Huacc. induction Huacc; eauto using access.
-Qed.
-
-(* ------------------------------------------------------------------------- *)
-(* not-unsafe-access preservation                                            *)
-(* ------------------------------------------------------------------------- *)
-
-Local Lemma nuacc_subst_preservation : forall m t tx ad x,
-  ~ unsafe_access ad m t ->
-  ~ unsafe_access ad m tx ->
-  ~ unsafe_access ad m ([x := tx] t).
-Proof.
-  intros. intros ?. induction t; eauto; simpl in *;
-  try (destruct string_eq_dec; eauto);
-  inv_uacc; inv_nuacc; eauto.
-Qed.
-
-Lemma nuacc_mem_add_preservation  : forall m t ad vT,
-  ~ unsafe_access (#m) m t ->
-  ~ unsafe_access ad m t ->
-  ~ unsafe_access ad (m +++ vT) t.
-Proof.
-  intros. intros Huacc. induction Huacc; inv_nuacc; eauto using unsafe_access.
-  decompose sum (lt_eq_lt_dec ad' (#m)); subst; simpl_array; simpl in *;
-  try inv_uacc; eauto using unsafe_access.
-  assert (#m <> ad') by eauto using Nat.lt_neq, Nat.neq_sym.
-  inv_nuacc. eauto.
-Qed.
-
-Lemma nuacc_mem_set_preservation : forall m t ad ad' v T,
-  ~ unsafe_access ad m v ->
-  ~ unsafe_access ad m t ->
-  ~ unsafe_access ad m[ad' <- (v, T)] t.
-Proof.
-  assert (forall m ad ad' v T,
-    unsafe_access ad m[ad' <- (v, T)] m[ad' <- (v, T)][ad'].tm -> ad' < #m). {
-      intros * H. eapply not_ge. rewrite ge_iff_le. intros ?.
-      rewrite (get_set_invalid memory_default) in H; trivial. inversion H.
-  }
-  (* main proof *)
-  intros * ? ? Huacc. induction Huacc; eauto using unsafe_access.
-  match goal with _ : _ <> ?ad |- _ => rename ad into ad'' end. 
-  destruct (nat_eq_dec ad' ad''); subst;
-  try (assert (ad'' < #m) by eauto);
-  simpl_array; eauto using unsafe_access.
-Qed.
-
-(* alternative for mem_set ------------------------------------------------- *)
-
-Lemma alt_nuacc_mem_set_preservation : forall m t ad ad' vT,
-  ~ unsafe_access ad' m t ->
-  ~ unsafe_access ad m t ->
-  ~ unsafe_access ad m[ad' <- vT] t.
-Proof.
-  intros * ? ? Huacc.
-  induction Huacc; inv_nuacc;
-  try solve [inv_nuacc; eauto].
-  match goal with Hneq : _ <> ?ad |- _ =>
-    destruct (nat_eq_dec ad' ad); subst
-  end; inv_nuacc. simpl_array. eauto.
-Qed.
-
-(* tstep ------------------------------------------------------------------- *)
-
-Lemma nuacc_tstep_none_preservation : forall m t t' ad,
-  ~ unsafe_access ad m t ->
-  t --[EF_None]--> t' ->
-  ~ unsafe_access ad m t'.
-Proof.
-  intros. induction_step; inv_nuacc; trivial;
-  try solve [do 2 auto_specialize; intros ?; inv_uacc; eauto].
-  inv_nuacc. eauto using nuacc_subst_preservation. 
-Qed.
-
-Lemma nuacc_tstep_alloc_preservation : forall m t t' ad v T,
-  ad < #m ->
-  forall_memory m (valid_addresses m) ->
-  valid_addresses m t ->
-  ~ unsafe_access ad m t ->
-  t --[EF_Alloc (#m) v T]--> t' ->
-  ~ unsafe_access ad (m +++ (v, T)) t'.
-Proof.
-  intros. intros ?. induction_step; inversion_vad; inv_nuacc; inv_clear_uacc;
-  eauto; try lia;
-  match goal with F : unsafe_access _ (_ +++ _) _ |- _ => contradict F end;
-  try simpl_array;
-  eauto using nacc_vad_length, nuacc_from_nacc, nuacc_mem_add_preservation.
-Qed.
-
-Lemma nuacc_tstep_read_preservation : forall m t t' ad ad' T,
-  forall_memory m value ->
-  empty |-- t is T ->
-  consistently_typed_references m t ->
-  ~ unsafe_access ad m t ->
-  t --[EF_Read ad' m[ad'].tm]--> t' ->
-  ~ unsafe_access ad m t'.
-Proof.
-  intros. intros ?. generalize dependent T.
-  induction_step; intros;
-  inversion_type; inversion_ctr; inv_nuacc; try inv_clear_uacc; eauto;
-  inversion_type; destruct (nat_eq_dec ad' ad); subst;
-  eauto using unsafe_access;
-  inversion_ctr;
-  match goal with F : unsafe_access _ _ _[_].tm |- _ => contradict F end;
-  eauto using immutable_reference_then_nuacc.
-Qed.
-
-Lemma nuacc_tstep_write_preservation : forall m t t' ad ad' v T,
-  ~ unsafe_access ad m t ->
-  t --[EF_Write ad' v T]--> t' ->
-  ~ unsafe_access ad m[ad' <- (v, T)] t'.
-Proof.
-  assert (forall m t t' ad ad' v T,
-    ~ unsafe_access ad m t ->
-    t --[EF_Write ad' v T]--> t' ->
-    ~ unsafe_access ad m v)
-    by (intros; induction_step; eauto using unsafe_access).
-  (* main proof *)
-  intros. intros ?. induction_step; inv_nuacc; inv_clear_uacc; eauto;
-  match goal with _ : unsafe_access _ _ ?t |- _ => rename t into tx end;
-  eapply (nuacc_mem_set_preservation _ tx _ _ v); eauto.
-Qed.
-
-Lemma nuacc_tstep_spawn_preservation : forall m t t' ad block,
-  ~ unsafe_access ad m t ->
-  t --[EF_Spawn block]--> t' ->
-  ~ unsafe_access ad m t'.
-Proof.
-  intros. intros ?. induction_step; try inv_nuacc; inv_uacc; eauto.
-Qed.
-
-Local Corollary nuacc_mstep_preservation : forall m m' t t' e ad T,
-  forall_memory m value ->
-  forall_memory m (valid_addresses m) ->
-  valid_addresses m t ->
-  empty |-- t is T ->
-  consistently_typed_references m t ->
-  (* --- *)
-  ad < #m ->
-  ~ unsafe_access ad m t ->
-  m / t ==[e]==> m' / t' ->
-  ~ unsafe_access ad m' t'.
-Proof.
-  intros. inversion_mstep;
-  eauto using nuacc_tstep_none_preservation,
-    nuacc_tstep_alloc_preservation,
-    nuacc_tstep_read_preservation,
-    nuacc_tstep_write_preservation.
-Qed.
-
-(* ------------------------------------------------------------------------- *)
-(*                                                                           *)
-(* ------------------------------------------------------------------------- *)
-
-Lemma memtyp_mstep_nuacc_then_immut : forall m m' t t' e T,
-  empty |-- t is T ->
-  (* --- *)
-  m / t ==[e]==> m' / t' ->
-  #m' > #m ->
-  ~ unsafe_access (#m) m' t' ->
-  exists Tm, m'[#m].typ = <{{i&Tm}}>.
-Proof.
-  intros * ? ? Hlen. intros. inversion_clear_mstep;
-  try rewrite set_preserves_length in Hlen; try lia.
-  simpl_array. simpl. generalize dependent T.
-  induction_step; intros; inversion_type; try inv_nuacc; eauto;
-  try match goal with
-  | _ : ?t --[_]--> _ , H : _ |-- ?t is _ |- _ =>
-    specialize (IHtstep _ H) as [? ?]; eauto
-  end.
-Qed.
-
-Lemma memtyp_mstep_uacc_then_mut : forall m m' t t' e T,
-  valid_accesses m t ->
-  empty |-- t is T ->
-  (* --- *)
-  m / t ==[e]==> m' / t' ->
-  #m' > #m ->
-  unsafe_access (#m) m' t' ->
-  exists Tm, m'[#m].typ = <{{&Tm}}>.
-Proof.
-  intros * ? ? ? Hlen. intros. inversion_clear_mstep;
-  try rewrite set_preserves_length in Hlen; try lia.
-  simpl_array. simpl. generalize dependent T.
-  induction_step; intros; inv_vac; inversion_type; try inv_clear_uacc;
-  eauto; exfalso;
-  match goal with
-  | H : valid_accesses _ ?t, _ : unsafe_access _ _ ?t |- _ =>
-    assert (~ access (#m) m t) by (intros F; specialize (H (#m) F); lia)
-  end;
-  eauto using uacc_then_acc, uacc_mem_add_inheritance.
-Qed.
 
