ValidAddresses.v
@@ -1,48 +1,19 @@
-From Coq Require Import Arith.Arith.
-From Coq Require Import Lia.
-
 From Elo Require Import Util.
 From Elo Require Import Array.
 From Elo Require Import Core.
-From Elo Require Import CoreExt.
 From Elo Require Import AnyTerm.
-From Elo Require Import Meta.
 
 (* ------------------------------------------------------------------------- *)
-(* has_address                                                               *)
+(* is-address & has-address                                                  *)
 (* ------------------------------------------------------------------------- *)
-
-(* TODO: make into submodule. *)
 
 Inductive is_address : addr -> tm -> Prop :=
-  | is_ad : forall ad T,
+  | is_address_constructor : forall ad T,
     is_address ad <{ &ad :: T}>
   .
 
 Notation "t 'has_address' ad" := (anyt (is_address ad) t)
   (at level 80, no associativity).
-
-Local Lemma write_requires_has_address : forall t t' ad v V,
-  t --[EF_Write ad v V]--> t' ->
-  t has_address ad.
-Proof.
-  intros. induction_step; eauto using anyt, is_address.
-Qed.
-
-Local Ltac inversion_is_address := 
-  match goal with
-  | H : is_address _ _ |- _ => inv_clear H
-  end.
-
-Local Ltac inversion_has_address := 
-  match goal with
-  | H : _ has_address _ |- _ =>
-      inv_clear H; try inversion_is_address
-  end.
-
-Local Hint Extern 4 =>
-  try inversion_has_address; try inversion_is_address
-  : has_address_inversion.
 
 (* ------------------------------------------------------------------------- *)
 (* valid-addresses                                                           *)
@@ -52,14 +23,8 @@ Local Hint Extern 4 =>
 Definition valid_addresses (m : mem) (t : tm) :=
   forall ad, t has_address ad -> ad < #m.
 
-Theorem valid_address_write : forall m t t' ad v V,
-  valid_addresses m t ->
-  t --[EF_Write ad v V]--> t' ->
-  ad < #m.
-Proof. eauto using write_requires_has_address. Qed.
-
 (* ------------------------------------------------------------------------- *)
-(* hints                                                                     *)
+(* unfold hints                                                              *)
 (* ------------------------------------------------------------------------- *)
 
 #[export] Hint Unfold valid_addresses : vad.
@@ -67,317 +32,147 @@ Proof. eauto using write_requires_has_address. Qed.
 #[export] Hint Extern 4 => unfold valid_addresses : vad.
 
 (* ------------------------------------------------------------------------- *)
-(* constructors                                                              *)
+(* is-address & has-address inversion                                        *)
 (* ------------------------------------------------------------------------- *)
 
-Local Lemma vad_unit : forall m,
-  valid_addresses m <{ unit }>.
-Proof. eauto with has_address_inversion vad. Qed.
+Local Ltac inv_isad := 
+  match goal with
+  | H : is_address _ _ |- _ => inv_clear H
+  end.
 
-Local Lemma vad_num : forall m n,
-  valid_addresses m <{ N n }>.
-Proof. eauto with has_address_inversion vad. Qed.
-
-Local Lemma vad_new : forall m t T,
-  valid_addresses m t ->
-  valid_addresses m <{ new T t }>.
-Proof. eauto with has_address_inversion vad. Qed.
-
-Local Lemma vad_load : forall m t,
-  valid_addresses m t ->
-  valid_addresses m <{ *t }>.
-Proof. eauto with has_address_inversion vad. Qed.
-
-Local Lemma vad_asg : forall m t1 t2,
-  valid_addresses m t1 ->
-  valid_addresses m t2 ->
-  valid_addresses m <{ t1 = t2 }>.
-Proof. eauto with has_address_inversion vad. Qed.
-
-Local Lemma vad_var : forall m x,
-  valid_addresses m <{ var x }>.
-Proof. eauto with has_address_inversion vad. Qed.
-
-Local Lemma vad_fun : forall m x Tx t,
-  valid_addresses m t ->
-  valid_addresses m <{ fn x Tx t }>.
-Proof. eauto with has_address_inversion vad. Qed.
-
-Local Lemma vad_call : forall m t1 t2,
-  valid_addresses m t1 ->
-  valid_addresses m t2 ->
-  valid_addresses m <{ call t1 t2 }>.
-Proof. eauto with has_address_inversion vad. Qed.
-
-Local Lemma vad_seq : forall m t1 t2,
-  valid_addresses m t1 ->
-  valid_addresses m t2 ->
-  valid_addresses m <{ t1; t2 }>.
-Proof. eauto with has_address_inversion vad. Qed.
-
-Local Lemma vad_spawn : forall m t,
-  valid_addresses m t ->
-  valid_addresses m <{ spawn t }>.
-Proof. eauto with has_address_inversion vad. Qed.
-
-Local Hint Resolve
-  vad_unit vad_num 
-  vad_new vad_load vad_asg
-  vad_var vad_fun vad_call vad_seq vad_spawn
-  : vad_constructors.
+Local Ltac inv_hasad := 
+  match goal with
+  | H : _ has_address _ |- _ =>
+      inv_clear H; try inv_isad
+  end.
 
 (* ------------------------------------------------------------------------- *)
-(* inversion                                                                 *)
+(* valid-addresses inversion                                                 *)
 (* ------------------------------------------------------------------------- *)
 
 Local Ltac solve_vad_inversion := 
   intros; try split; eauto using anyt, is_address with vad.
 
-(* vad_unit implicates nothing *)
-(* vad_num implicates nothing *)
-
 Local Lemma inv_vad_ref : forall m ad T,
-  valid_addresses m <{ &ad :: T }> ->
+  valid_addresses m <{&ad :: T}> ->
   ad < #m.
 Proof. solve_vad_inversion. Qed.
 
 Local Lemma inv_vad_new : forall m t T,
-  valid_addresses m <{ new T t }> ->
+  valid_addresses m <{new T t}> ->
   valid_addresses m t.
 Proof. solve_vad_inversion. Qed.
 
 Local Lemma inv_vad_load : forall m t,
-  valid_addresses m <{ *t }> ->
+  valid_addresses m <{*t}> ->
   valid_addresses m t.
 Proof. solve_vad_inversion. Qed.
 
 Local Lemma inv_vad_asg : forall m t1 t2,
-  valid_addresses m <{ t1 = t2 }> ->
+  valid_addresses m <{t1 = t2}> ->
   valid_addresses m t1 /\ valid_addresses m t2.
 Proof. solve_vad_inversion. Qed.
 
-(* vad_var implicates nothing *)
-
 Local Lemma inv_vad_fun : forall m x Tx t,
-  valid_addresses m <{ fn x Tx t }> ->
+  valid_addresses m <{fn x Tx t}> ->
   valid_addresses m t.
 Proof. solve_vad_inversion. Qed.
 
 Local Lemma inv_vad_call : forall m t1 t2,
-  valid_addresses m <{ call t1 t2 }> ->
+  valid_addresses m <{call t1 t2}> ->
   valid_addresses m t1 /\ valid_addresses m t2.
 Proof. solve_vad_inversion. Qed.
 
 Local Lemma inv_vad_seq : forall m t1 t2,
-  valid_addresses m <{ t1; t2 }> ->
+  valid_addresses m <{t1; t2}> ->
   valid_addresses m t1 /\ valid_addresses m t2.
 Proof. solve_vad_inversion. Qed.
 
 Local Lemma inv_vad_spawn : forall m t,
-  valid_addresses m <{ spawn t }> ->
+  valid_addresses m <{spawn t}> ->
   valid_addresses m t.
 Proof. solve_vad_inversion. Qed.
 
-Ltac inversion_vad :=
+Ltac inv_vad :=
  match goal with
- | H: valid_addresses _ <{ & _ :: _ }> |- _ => eapply inv_vad_ref  in H as ?
- | H: valid_addresses _ <{ new _ _  }> |- _ => eapply inv_vad_new  in H
- | H: valid_addresses _ <{ * _      }> |- _ => eapply inv_vad_load in H
- | H: valid_addresses _ <{ _ = _    }> |- _ => eapply inv_vad_asg  in H as [? ?]
- | H: valid_addresses _ <{ fn _ _ _ }> |- _ => eapply inv_vad_fun  in H
- | H: valid_addresses _ <{ call _ _ }> |- _ => eapply inv_vad_call in H as [? ?]
- | H: valid_addresses _ <{ _ ; _    }> |- _ => eapply inv_vad_seq  in H as [? ?]
- | H: valid_addresses _ <{ spawn _  }> |- _ => eapply inv_vad_spawn in H
+ (* irrelevant for unit *)
+ (* irrelevant for num  *)
+ | H : valid_addresses _ <{& _ :: _}> |- _ => eapply inv_vad_ref   in H as ?
+ | H : valid_addresses _ <{new _ _ }> |- _ => eapply inv_vad_new   in H
+ | H : valid_addresses _ <{* _     }> |- _ => eapply inv_vad_load  in H
+ | H : valid_addresses _ <{_ = _   }> |- _ => eapply inv_vad_asg   in H as [? ?]
+ (* irrelevant for var  *)
+ | H : valid_addresses _ <{fn _ _ _}> |- _ => eapply inv_vad_fun   in H
+ | H : valid_addresses _ <{call _ _}> |- _ => eapply inv_vad_call  in H as [? ?]
+ | H : valid_addresses _ <{_ ; _   }> |- _ => eapply inv_vad_seq   in H as [? ?]
+ | H : valid_addresses _ <{spawn _ }> |- _ => eapply inv_vad_spawn in H
  end.
 
 (* ------------------------------------------------------------------------- *)
-(* preservation                                                              *)
+(* valid-addresses construction                                              *)
 (* ------------------------------------------------------------------------- *)
 
-Local Lemma vad_subst_preservation : forall m t tx x,
+Local Ltac solve_vad_construction := 
+  intros ** ? ?; inv_hasad; eauto.
+
+Local Lemma vad_unit : forall m,
+  valid_addresses m <{unit}>.
+Proof. solve_vad_construction. Qed.
+
+Local Lemma vad_num : forall m n,
+  valid_addresses m <{N n}>.
+Proof. solve_vad_construction. Qed.
+
+Local Lemma vad_ad : forall m ad T,
+  ad < #m ->
+  valid_addresses m <{&ad :: T}>.
+Proof. solve_vad_construction. Qed.
+
+Local Lemma vad_new : forall m t T,
   valid_addresses m t ->
-  valid_addresses m tx ->
-  valid_addresses m ([x := tx] t).
-Proof.
-  intros. induction t; try inversion_vad; simpl; eauto with vad_constructors;
-  destruct string_eq_dec; subst; trivial;
-  autounfold with vad in *; eauto with has_address_inversion.
-Qed.
+  valid_addresses m <{new T t}>.
+Proof. solve_vad_construction. Qed.
 
-Local Lemma vad_mem_add_preservation : forall m t vT,
+Local Lemma vad_load : forall m t,
   valid_addresses m t ->
-  valid_addresses (m +++ vT) t.
-Proof.
-  intros. intros ? Hha. rewrite add_increments_length.
-  induction Hha; try inversion_vad; eauto with has_address_inversion.
-Qed.
+  valid_addresses m <{*t}>.
+Proof. solve_vad_construction. Qed.
 
-Local Lemma vad_mem_set_preservation : forall m t ad vT,
+Local Lemma vad_asg : forall m t1 t2,
+  valid_addresses m t1 ->
+  valid_addresses m t2 ->
+  valid_addresses m <{t1 = t2}>.
+Proof. solve_vad_construction. Qed.
+
+Local Lemma vad_var : forall m x,
+  valid_addresses m <{var x}>.
+Proof. solve_vad_construction. Qed.
+
+Local Lemma vad_fun : forall m x Tx t,
   valid_addresses m t ->
-  valid_addresses m[ad <- vT] t.
-Proof.
-  intros. intros ? Hha. rewrite set_preserves_length.
-  induction Hha; try inversion_vad; eauto with has_address_inversion.
-Qed.
+  valid_addresses m <{fn x Tx t}>.
+Proof. solve_vad_construction. Qed.
 
-(* ------------------------------------------------------------------------- *)
+Local Lemma vad_call : forall m t1 t2,
+  valid_addresses m t1 ->
+  valid_addresses m t2 ->
+  valid_addresses m <{call t1 t2}>.
+Proof. solve_vad_construction. Qed.
 
-Local Lemma vad_tstep_none_preservation : forall m t t',
+Local Lemma vad_seq : forall m t1 t2,
+  valid_addresses m t1 ->
+  valid_addresses m t2 ->
+  valid_addresses m <{t1; t2}>.
+Proof. solve_vad_construction. Qed.
+
+Local Lemma vad_spawn : forall m t,
   valid_addresses m t ->
-  t --[EF_None]--> t' ->
-  valid_addresses m t'.
-Proof.
-  intros. induction_step; inversion_vad; eauto with vad_constructors. 
-  inversion_vad. eauto using vad_subst_preservation.
-Qed.
+  valid_addresses m <{spawn t}>.
+Proof. solve_vad_construction. Qed.
 
-Local Lemma vad_tstep_alloc_preservation : forall m t t' v T,
-  valid_addresses m t ->
-  t --[EF_Alloc (#m) v T]--> t' ->
-  valid_addresses (m +++ (v, T)) t'.
-Proof.
-  intros. induction_step; inversion_vad;
-  eauto using vad_mem_add_preservation with vad_constructors.
-  intros ? ?. inversion_has_address. rewrite add_increments_length. eauto.
-Qed.
-
-Local Lemma vad_tstep_read_preservation : forall m t t' ad v,
-  valid_addresses m v ->
-  valid_addresses m t ->
-  t --[EF_Read ad v]--> t' ->
-  valid_addresses m t'.
-Proof.
-  intros. induction_step; inversion_vad; eauto with vad_constructors.
-Qed.
-
-Local Lemma vad_tstep_write_preservation : forall m t t' ad v T,
-  valid_addresses m t ->
-  t --[EF_Write ad v T]--> t' ->
-  valid_addresses m[ad <- (v, T)] t'.
-Proof.
-  intros. assert (valid_addresses m v); induction_step; inversion_vad;
-  eauto using vad_mem_set_preservation with vad_constructors.
-Qed.
-
-Local Lemma vad_tstep_spawn_preservation : forall m t t' block,
-  valid_addresses m t ->
-  t --[EF_Spawn block]--> t' ->
-  valid_addresses m t'.
-Proof.
-  intros. induction_step; inversion_vad; eauto with vad_constructors.
-Qed.
-
-Local Corollary vad_mstep_preservation : forall m m' t t' e,
-  forall_memory m (valid_addresses m) ->
-  valid_addresses m t ->
-  m / t ==[e]==> m' / t' ->
-  valid_addresses m' t'.
-Proof.
-  solve_mstep_preservation_using
-    vad_tstep_none_preservation
-    vad_tstep_alloc_preservation
-    vad_tstep_read_preservation
-    vad_tstep_write_preservation.
-Qed.
-
-(* ------------------------------------------------------------------------- *)
-
-Local Lemma vad_thread_default_preservation : forall m,
-  valid_addresses m thread_default.
-Proof.
-  intros. eauto with vad_constructors.
-Qed.
-
-Local Lemma vad_spawn_block_preservation : forall m t t' block,
-  valid_addresses m t ->
-  t --[EF_Spawn block]--> t' ->
-  valid_addresses m block.
-Proof.
-  intros. induction_step; inversion_vad; eauto.
-Qed.
-
-Local Lemma vad_untouched_threads_preservation : forall m m' ths tid tid' e t',
-  forall_threads ths (valid_addresses m) ->
-  tid <> tid' ->
-  tid' < #ths ->
-  m / ths[tid] ==[e]==> m' / t' ->
-  valid_addresses m' ths[tid'].
-Proof.
-  intros. intros ? ?. autounfold with vad in *. inversion_mstep; eauto;
-  (rewrite add_increments_length || rewrite set_preserves_length);
-  eauto using Nat.lt_lt_succ_r.
-Qed.
-
-Corollary vad_cstep_preservation : forall m m' ths ths' tid e,
-  forall_memory m (valid_addresses m) ->
-  forall_threads ths (valid_addresses m) ->
-  m / ths ~~[tid, e]~~> m' / ths' ->
-  forall_threads ths' (valid_addresses m').
-Proof.
-  eauto 6 using cstep_preservation,
-    vad_tstep_spawn_preservation,
-    vad_mstep_preservation,
-    vad_thread_default_preservation,
-    vad_spawn_block_preservation,
-    vad_untouched_threads_preservation.
-Qed.
-
-(* ------------------------------------------------------------------------- *)
-
-Local Lemma vad_tstep_alloc_mem_preservation : forall m t t' v T,
-  valid_addresses m t ->
-  forall_memory m (valid_addresses m) ->
-  t --[EF_Alloc (#m) v T]--> t' ->
-  forall_memory  (m +++ (v, T)) (valid_addresses (m +++ (v, T))).
-Proof.
-  intros. intros ad.
-  decompose sum (lt_eq_lt_dec ad (#m)); subst; simpl_array;
-  intros ? ?; rewrite add_increments_length; autounfold with vad in *;
-  eauto using anyt_alloc_generalization, Nat.lt_lt_succ_r
-        with has_address_inversion.
-Qed.
-
-Local Lemma vad_tstep_write_mem_preservation : forall m t t' ad v T,
-  valid_addresses m t ->
-  forall_memory m (valid_addresses m) ->
-  t --[EF_Write ad v T]--> t' ->
-  forall_memory m[ad <- (v, T)] (valid_addresses m[ad <- (v, T)]).
-Proof.
-  intros. intros ad'. 
-  assert (ad < #m) by eauto using valid_address_write.
-  destruct (eq_nat_dec ad ad'); subst; simpl_array;
-  intros ? ?; rewrite set_preserves_length; autounfold with vad in *;
-  eauto using anyt_write_generalization, Nat.lt_lt_succ_r.
-Qed.
-
-Local Corollary vad_mstep_mem_preservation : forall m m' t t' e,
-  valid_addresses m t ->
-  forall_memory m (valid_addresses m) ->
-  m / t ==[e]==> m' / t' ->
-  forall_memory m' (valid_addresses m').
-Proof.
-  solve_mstep_mem_preservation_using 
-    vad_tstep_alloc_mem_preservation 
-    vad_tstep_write_mem_preservation.
-Qed.
-
-Local Corollary vad_cstep_mem_preservation : forall m m' ths ths' tid e,
-  forall_threads ths (valid_addresses m) ->
-  forall_memory m (valid_addresses m) ->
-  m / ths ~~[tid, e]~~> m' / ths' ->
-  forall_memory m' (valid_addresses m').
-Proof.
-  solve_cstep_mem_preservation_using vad_mstep_mem_preservation.
-Qed.
-
-(* ------------------------------------------------------------------------- *)
-
-Theorem valid_addresses_preservation : forall m m' ths ths' tid e,
-  forall_program m ths (valid_addresses m) ->
-  m / ths ~~[tid, e]~~> m' / ths' ->
-  forall_program m' ths' (valid_addresses m').
-Proof.
-  intros * [? ?]. intros.
-  eauto using vad_cstep_preservation, vad_cstep_mem_preservation.
-Qed.
+#[export] Hint Resolve
+  vad_unit vad_num
+  vad_ad vad_new vad_load vad_asg
+  vad_var vad_fun vad_call vad_seq vad_spawn
+  : vad.
 
