WellTypedTerm.v
@@ -1,0 +1,6 @@
+From Elo Require Import Map.
+From Elo Require Import Core.
+
+Definition well_typed_term (t : tm) :=
+  exists T, empty |-- t is T.
+
